coq-osiris/theories/program_logic/pure/wp.v
@@ -912,6 +912,7 @@ Section pure_wp_rules.
       inv Hstep; eauto with may.
       + by apply invert_pure_wp_stop in Hm.
       + by apply invert_pure_wp_stop in Hm.
+      + by apply invert_pure_wp_stop in Hm.
       + edestruct IHm; eauto with may.
     - pose proof invert_pure_wp_stop _ _ _ _ _ Hm.
       destruct c; try tauto; invdep Hstep; split; auto; try destruct b; constructor.
@@ -919,6 +920,8 @@ Section pure_wp_rules.
       pose proof invert_pure_wp_Par_right _ _ _ Hm as Hm2.
       invdep Hstep; try (split; [ | tauto ]).
       all: try by constructor.
+      + by apply invert_pure_wp_stop in Hm1.
+      + by apply invert_pure_wp_stop in Hm2.
       + by apply invert_pure_wp_stop in Hm1.
       + by apply invert_pure_wp_stop in Hm2.
       + by apply invert_pure_wp_stop in Hm1.
@@ -948,6 +951,7 @@ Section pure_wp_rules.
       + by apply invert_pure_wp_throw in Hm.
       + by apply invert_pure_wp_stop in Hm.
       + by apply invert_pure_wp_stop in Hm.
+      + by apply invert_pure_wp_stop in Hm.
       + by apply invert_pure_wp_crash in Hm.
       + edestruct IHm as [IH ->]; eauto. split; auto.
         eapply pure_wp_handle; eauto.
@@ -958,6 +962,8 @@ Section pure_wp_rules.
       pose proof invert_pure_wp_Par_right _ _ _ Hm as Hm2.
       invdep Hstep; try (split; [ | tauto ]).
       all: eauto using pure_wp_may_forward with may.
+      + by apply invert_pure_wp_stop in Hm1.
+      + by apply invert_pure_wp_stop in Hm2.
       + by apply invert_pure_wp_stop in Hm1.
       + by apply invert_pure_wp_stop in Hm2.
       + by apply invert_pure_wp_stop in Hm1.
@@ -1028,7 +1034,9 @@ Section pure_wp_rules.
       intros P. apply pure_wp_Par; eauto with pure.
     - (* Stop CPerf is impure_wp *)
       intros []%invert_pure_wp_stop.
-    - (* Stop CPerf is impure_wp *)
+    - (* Stop CFork is impure_wp *)
+      intros []%invert_pure_wp_stop.
+    - (* Stop CJoin is impure_wp *)
       intros []%invert_pure_wp_stop.
     - intros P. apply pure_wp_handle, IHS. by constructor.
     - intros P. apply pure_wp_handle, IHS. by constructor.
@@ -1053,6 +1061,7 @@ Section pure_wp_rules.
       apply pure_wp_Par; eapply pure_wp_mono_ret; eauto; firstorder eauto.
     - (* SimpParThrowAgree uses only one hyp *)
       by intros P%invert_pure_wp_Par_left%IHS1%invert_pure_wp_throw.
+    - intros []%invert_pure_wp_stop.
     - intros []%invert_pure_wp_stop.
     - intros []%invert_pure_wp_stop.
     - by intros P%invert_pure_wp_handle%IHS%invert_pure_wp_ret.
